veric/mem_lessdef.v
@@ -8,7 +8,6 @@ Require Import compcert.common.Values.
 
 Require Import VST.msl.Coqlib2.
 Require Import VST.msl.eq_dec.
-Require Import VST.msl.seplog.
 Require Import VST.veric.Memory.
 Require Import VST.veric.juicy_mem.
 
@@ -59,8 +58,8 @@ Proof.
     { rewrite E; tauto. } clear E.
     specialize (S b ofs k). revert S.
     unfold access_at, Mem.perm. simpl.
-    set (o1 := (Mem.mem_access _) !! b ofs k).
-    set (o2 := (Mem.mem_access _) !! b ofs k). clearbody o1 o2. intros S.
+    set (o1 := (Maps.PMap.get b (Mem.mem_access _) ofs k)).
+    set (o2 := (Maps.PMap.get b (Mem.mem_access _) ofs k)). clearbody o1 o2. intros S.
     assert (S' : forall o, Mem.perm_order'' o1 o <-> Mem.perm_order'' o2 o).
     { intros [ o | ]. apply S. destruct o1 as [o1 | ], o2 as [o2 | ]; split; intro; constructor. }
     clear S.
@@ -87,7 +86,7 @@ Proof.
     unfold Mem.loadbytes in *.
     apply equal_f with (x := b) in E.
     apply equal_f with (x := ofs) in E.
-    apply equal_f with (x := 1) in E.
+    apply equal_f with (x := 1%Z) in E.
     unfold access_at in *.
     if_tac [p1|np1] in E; if_tac in E; try discriminate.
     + simpl in E.
@@ -192,7 +191,7 @@ Proof.
     f_equal; auto.
     apply memval_lessdef_antisym; auto.
   - repeat extensionality.
-    apply prop_ext; split; auto.
+    apply Axioms.prop_ext; split; auto.
   - zify.
     cut (Z.pos (Mem.nextblock m2) = Z.pos (Mem.nextblock m1)).
     congruence. lia.
@@ -290,7 +289,7 @@ Lemma mem_lessdef_weak_valid_pointer:
 Proof.
 intros.
 unfold Mem.weak_valid_pointer in *.
-rewrite orb_true_iff in *.
+rewrite -> orb_true_iff in *.
 destruct H0; [left|right]; eapply mem_lessdef_valid_pointer; eauto.
 Qed.
 
@@ -445,12 +444,13 @@ Proof.
   rewrite (valid_pointer_lessalloc M); trivial.
 Qed.
 
-
+(*
 Definition juicy_mem_equiv jm1 jm2 := mem_equiv (m_dry jm1) (m_dry jm2) /\ m_phi jm1 = m_phi jm2.
 
 Definition juicy_mem_lessdef jm1 jm2 := mem_lessdef (m_dry jm1) (m_dry jm2) /\ m_phi jm1 = m_phi jm2.
 
 Definition juicy_mem_lessalloc jm1 jm2 := mem_lessdef (m_dry jm1) (m_dry jm2) /\ m_phi jm1 = m_phi jm2.
+*)
 
 Ltac sync D :=
   first
